src/QueryStructure/Implementation/DataStructures/BagADT/QueryStructureImplementation.v
@@ -1,0 +1,79 @@
+Require Import Coq.Lists.List Coq.Program.Program
+        Coq.Bool.Bool Coq.Strings.String
+        Coq.Structures.OrderedTypeEx Coq.Arith.Arith
+        ADTSynthesis.Common.ilist
+        ADTSynthesis.Common.i2list
+        ADTSynthesis.Computation
+        ADTSynthesis.ADT
+        ADTSynthesis.ADTRefinement
+        ADTSynthesis.ADTNotation
+        ADTSynthesis.QueryStructure.Specification.Representation.QueryStructureSchema
+        ADTSynthesis.QueryStructure.Specification.Representation.QueryStructure
+        ADTSynthesis.QueryStructure.Implementation.DataStructures.BagADT.BagADT.
+
+Section QueryStructureImplementation.
+
+  Variable qs_schema : QueryStructureSchema.
+
+  (* Build an index requires search terms and matchers for each schema,
+     and update terms and updaters for each schema. *)
+
+  Record SearchUpdateTerms (heading : Heading) :=
+    {  BagSearchTermType : Type;
+       BagMatchSearchTerm : BagSearchTermType -> @Tuple heading -> bool;
+       BagUpdateTermType : Type;
+       BagApplyUpdateTerm : BagUpdateTermType -> @Tuple heading -> @Tuple heading }.
+
+  Variable BagIndexKeys :
+    ilist (fun ns => SearchUpdateTerms (schemaHeading (relSchema ns)))
+      (qschemaSchemas qs_schema).
+
+  Definition IndexedQueryStructure
+    := i2list (A := NamedSchema)
+              (fun ns index => Rep (BagSpec (BagMatchSearchTerm index)
+                                            (BagApplyUpdateTerm index)))
+              BagIndexKeys.
+
+  Definition GetIndexedRelation (r_n : IndexedQueryStructure) idx
+    := i2th_Bounded relName r_n idx.
+
+  Definition CallBagMethod idx midx r_n :=
+    Methods (BagSpec (BagMatchSearchTerm (ith_Bounded relName BagIndexKeys idx))
+                     (BagApplyUpdateTerm (ith_Bounded relName BagIndexKeys idx)))
+            midx
+            (GetIndexedRelation r_n idx).
+
+  Definition CallBagConstructor idx midx :=
+    Constructors (BagSpec (BagMatchSearchTerm (ith_Bounded relName BagIndexKeys idx))
+                          (BagApplyUpdateTerm (ith_Bounded relName BagIndexKeys idx)))
+            midx.
+
+  Definition DelegateToBag_AbsR
+             (r_o : UnConstrQueryStructure qs_schema)
+             (r_n : IndexedQueryStructure)
+    := forall idx, GetUnConstrRelation r_o idx = GetIndexedRelation r_n idx.
+
+  Fixpoint Initialize_IndexedQueryStructure
+          (ns : list NamedSchema)
+          (indices' : ilist (fun ns => SearchUpdateTerms (schemaHeading (relSchema ns))) ns)
+          {struct indices'}
+  : Comp (i2list (fun ns index =>
+                    Rep (BagSpec (BagMatchSearchTerm index)
+                                  (BagApplyUpdateTerm index))) indices')
+    := match indices' return Comp (i2list _ indices') with
+      | inil => ret (i2nil _ _)
+      | icons ns ns' index indices'' =>
+        c <- (Constructors
+                (BagSpec (BagMatchSearchTerm index) (BagApplyUpdateTerm index))
+                {|bindex := "EmptyBag" |} tt);
+          cs <- (@Initialize_IndexedQueryStructure ns' indices'');
+          ret (i2cons ns index c cs)
+
+    end.
+
+End QueryStructureImplementation.
+
+Opaque CallBagMethod.
+Arguments CallBagMethod : simpl never.
+Opaque CallBagConstructor.
+Arguments CallBagConstructor : simpl never.
