src/QueryStructure/Specification/Operations/Update.v
@@ -1,11 +1,14 @@
 Require Import Coq.Lists.List Coq.Strings.String Coq.Sets.Ensembles Coq.Arith.Arith
         ADTSynthesis.Computation.Core
-        ADTSynthesis.ADT.ADTSig ADTSynthesis.ADT.Core
-        ADTSynthesis.Common.ilist ADTSynthesis.Common.StringBound ADTSynthesis.QueryStructure.IndexedEnsembles
-        ADTSynthesis.ADTNotation.BuildADT ADTSynthesis.ADTNotation.BuildADTSig
-        ADTSynthesis.QueryStructure.QueryStructureSchema ADTSynthesis.QueryStructure.QueryStructure
-        ADTSynthesis.QueryStructure.QuerySpecs.InsertQSSpecs
-        ADTSynthesis.QueryStructure.QuerySpecs.DeleteQSSpecs.
+        ADTSynthesis.ADT.ADTSig
+        ADTSynthesis.ADT.Core
+        ADTSynthesis.Common.ilist
+        ADTSynthesis.Common.StringBound
+        ADTSynthesis.Common.Ensembles.IndexedEnsembles
+        ADTSynthesis.ADTNotation.BuildADT
+        ADTSynthesis.ADTNotation.BuildADTSig
+        ADTSynthesis.QueryStructure.Specification.Representation.QueryStructureSchema
+        ADTSynthesis.QueryStructure.Specification.Representation.QueryStructure.
 
 (* Definitions for updating query structures. *)
 
