src/QueryStructure/Specification/Representation/QueryStructureNotations.v
@@ -4,6 +4,14 @@ Require Export Coq.Strings.String Coq.omega.Omega Coq.Lists.List Coq.Logic.Funct
         ADTSynthesis.ADTRefinement.BuildADTRefinements ADTSynthesis.QueryStructure.Specification.Operations.Query ADTSynthesis.QueryStructure.Specification.Operations.Insert ADTSynthesis.QueryStructure.Specification.Operations.Empty (* Add Update *)
         ADTSynthesis.QueryStructure.Specification.Operations.Delete ADTSynthesis.QueryStructure.Specification.Representation.QueryStructure.
 
+Notation "heading / attr_index" := ((fun x : Attributes heading => x)
+                                       {| bindex := attr_index; indexb := _ |})
+                                      (at level 40, left associativity) : QueryStructure_scope.
+
+Notation "QSSchema # rel_key" := (TupleDef QSSchema rel_key) (at level 100, no associativity) : QueryStructure_scope.
+
+Notation "?[ A ]" := (if A then true else false) (at level 50) : QueryStructure_scope.
+
 Open Scope QSSchema.
 Open Scope ADTSig.
 Open Scope QueryImpl.
